Install pp_X pretty-printers early in translation
Sets up the pp_data type and the initial pretty printers and
translates them immediately after decProg. Some of these can
be replaced later, as is already done for Vector.

Requires translating some of the toString functionality in
mlint earlier in the process. Some of those functions were
adjusted to be easier to translate.

Working up to IntProg, which is somehow broken by some of its
constants already being translated, or for some other mysterious
reason, shadowing induction theorems doesn't seem to be doing
what it should (or rather, what it previously did).

basis/IntProgScript.sml
@@ -26,46 +26,12 @@ val _ = trans "<=" intSyntax.leq_tm;
 val _ = trans ">=" intSyntax.geq_tm;
 val _ = trans "~" ``\i. - (i:int)``;
 
-val _ = ml_prog_update open_local_block;
-
-val result = translate zero_pad_def
-
-val result = translate toChar_def
-val tochar_side_def = definition"tochar_side_def";
-val tochar_side = Q.prove(
-  `∀x. tochar_side x <=> (~(x < 10) ==> x < 201)`,
-  rw[tochar_side_def])
-  |> update_precondition;
-
-val result = translate simple_toChars_def
-
-val simple_toChars_side = Q.prove(
-  `∀x y z. simple_tochars_side x y z = T`,
-  ho_match_mp_tac simple_toChars_ind \\ rw[]
-  \\ rw[Once (theorem"simple_tochars_side_def")])
-  |> update_precondition;
-
-val _ = save_thm("toChars_ind",
-   toChars_ind |> REWRITE_RULE[maxSmall_DEC_def,padLen_DEC_eq]);
-val _ = add_preferred_thy "-";
-val result = translate
-  (toChars_def |> REWRITE_RULE[maxSmall_DEC_def,padLen_DEC_eq]);
-
-val _ = ml_prog_update open_local_in_block;
+Definition rename_toString_def:
+  rename_toString = mlint$toString
+End
 
 val _ = next_ml_names := ["toString"];
-
-val toString_v_thm = translate
-  (toString_def |> REWRITE_RULE[maxSmall_DEC_def])
-val tostring_side = Q.prove(
-  `∀x. tostring_side x = T`,
-  rw[definition"tostring_side_def"]
-  \\ intLib.COOPER_TAC)
-  |> update_precondition;
-
-val toString_v_thm = toString_v_thm
-  |> DISCH_ALL |> REWRITE_RULE [tostring_side,ml_translatorTheory.PRECONDITION_def]
-  |> ml_translatorLib.remove_Eq_from_v_thm;
+val toString_v_thm = translate rename_toString_def;
 
 val Eval_NUM_toString = Q.prove(
   `!v. (INT --> STRING_TYPE) toString v ==>
@@ -74,7 +40,7 @@ val Eval_NUM_toString = Q.prove(
     ml_translatorTheory.AppReturns_def,num_to_str_def,
     ml_translatorTheory.NUM_def,PULL_EXISTS,FORALL_PROD]
   \\ rw [] \\ res_tac)
-  |> (fn th => MATCH_MP th toString_v_thm)
+  |> (fn th => MATCH_MP th (REWRITE_RULE [rename_toString_def] toString_v_thm))
   |> add_user_proved_v_thm;
 
 val _ = ml_prog_update open_local_block;
@@ -83,10 +49,10 @@ val th = EVAL``ORD #"0"``;
 val result = translate (fromChar_unsafe_def |> SIMP_RULE std_ss [th]);
 val result = translate fromChars_range_unsafe_def;
 
-val _ = save_thm("fromChars_unsafe_ind",
-  fromChars_unsafe_ind |> REWRITE_RULE[maxSmall_DEC_def,padLen_DEC_eq]);
-val result = translate (fromChars_unsafe_def
-  |> REWRITE_RULE[maxSmall_DEC_def,padLen_DEC_eq]);
+val result = translate padLen_DEC_eq;
+val result = translate maxSmall_DEC_def;
+
+val result = translate (fromChars_unsafe_def);
 
 val result = translate fromString_unsafe_def;
 
@@ -94,11 +60,20 @@ val fromstring_unsafe_side_def = definition"fromstring_unsafe_side_def";
 val fromchars_unsafe_side_def = theorem"fromchars_unsafe_side_def";
 val fromchars_range_unsafe_side_def = theorem"fromchars_range_unsafe_side_def";
 
+Theorem fromchars_range_unsafe_side_thm:
+   ∀j i s. i + j ≤ strlen s ⇒ fromchars_range_unsafe_side i j s
+Proof
+  Induct
+  \\ rw[Once fromchars_range_unsafe_side_def]
+QED
+
 Theorem fromchars_unsafe_side_thm:
    ∀n s. n ≤ LENGTH s ⇒ fromchars_unsafe_side n (strlit s)
 Proof
   completeInduct_on`n` \\ rw[]
-  \\ rw[Once fromchars_unsafe_side_def,fromchars_range_unsafe_side_def]
+  \\ rw[Once fromchars_unsafe_side_def, padLen_DEC_eq]
+  \\ irule fromchars_range_unsafe_side_thm
+  \\ simp []
 QED
 
 val fromString_unsafe_side = Q.prove(
@@ -122,10 +97,7 @@ QED
 val result = translate fromChar_thm;
 val result = translate fromChars_range_def;
 
-val _ = save_thm("fromChars_ind",
-  fromChars_ind |> REWRITE_RULE[maxSmall_DEC_def,padLen_DEC_eq]);
-val result = translate (fromChars_def
-  |> REWRITE_RULE[maxSmall_DEC_def,padLen_DEC_eq]);
+val result = translate fromChars_def;
 
 val _ = ml_prog_update open_local_in_block;
 
@@ -139,7 +111,7 @@ Theorem fromchars_side_thm:
    ∀n s. n ≤ LENGTH s ⇒ fromchars_side n (strlit s)
 Proof
   completeInduct_on`n` \\ rw[]
-  \\ rw[Once fromchars_side_def,fromchars_range_side_def]
+  \\ rw[Once fromchars_side_def,fromchars_range_side_def, padLen_DEC_eq]
 QED
 
 val fromString_side = Q.prove(
@@ -169,6 +141,8 @@ val gcd_side = prove(
   \\ once_rewrite_tac [theorem "gcd_side_def"]
   \\ fs [ADD1] \\ rw [] \\ fs [])
   |> update_precondition;
+
+theorem "gcd_ind" |> update_precondition
 
 (* compare *)
 
