translator/pp_setupScript.sml
@@ -1,0 +1,75 @@
+(*
+  Install manually defined components of the pretty-printer.
+
+  Once these components are present, the add-pretty-printer
+  pass has the resources it needs to define pretty printers
+  for additional types.
+*)
+
+open preamble astTheory semanticPrimitivesTheory;
+open ml_translatorLib ml_translatorTheory ml_progLib;
+open decProgTheory mlprettyprinterTheory;
+
+val _ = new_theory "pp_setup";
+
+val _ = translation_extends "decProg";
+
+val _ = register_type ``: pp_data``;
+
+fun def_of_const tm = let
+  val res = dest_thy_const tm handle HOL_ERR _ =>
+              failwith ("Unable to translate: " ^ term_to_string tm)
+  val name = (#Name res)
+  fun def_from_thy thy name =
+    DB.fetch thy (name ^ "_pmatch") handle HOL_ERR _ =>
+    DB.fetch thy (name ^ "_def") handle HOL_ERR _ =>
+    DB.fetch thy (name ^ "_DEF") handle HOL_ERR _ =>
+    DB.fetch thy name
+  val def = def_from_thy (#Thy res) name handle HOL_ERR _ =>
+            failwith ("Unable to find definition of " ^ name)
+  in def end;
+
+val _ = (find_def_for_const := def_of_const);
+
+val res = translate pp_fun_def;
+val res = translate pp_exn_def;
+val res = translate pp_paren_tuple_def;
+val res = translate pp_app_block_def;
+val res = translate pp_list_def;
+val res = translate pp_string_def;
+val res = translate pp_char_def;
+val res = translate pp_bool_def;
+
+(* useless pretty-printers for impure types. added here to ensure no type
+   errors. should be replaced later in the basis *)
+val res = translate pp_ref_def;
+val res = translate pp_array_def;
+val res = translate pp_word8array_def;
+val res = translate pp_vector_def;
+
+(* translate pps for numeric types, which are actually used early. *)
+val res = translate mlintTheory.num_to_rev_chars_def;
+
+Triviality tochar_side_dec:
+  i < 10 ==> tochar_side i
+Proof
+  EVAL_TAC \\ simp []
+QED
+
+Triviality num_to_rev_chars_side:
+  !i j k. num_to_rev_chars_side i j k
+Proof
+  ho_match_mp_tac mlintTheory.num_to_rev_chars_ind
+  \\ rw []
+  \\ ONCE_REWRITE_TAC [fetch "-" "num_to_rev_chars_side_def"]
+  \\ simp [tochar_side_dec]
+QED
+
+val res = update_precondition num_to_rev_chars_side;
+
+val res = translate pp_int_def;
+val res = translate pp_word8_def;
+val res = translate pp_word64_def;
+
+val _ = export_theory();
+
