translator/README.md
@@ -60,6 +60,9 @@ algorithms in "Purely Functional Data Structures" by Chris Okasaki (1996).
 [other-examples](other-examples):
 A few other examples of HOL functions that can be translated into CakeML.
 
+[pp_setupScript.sml](pp_setupScript.sml):
+Install manually defined components of the pretty-printer.
+
 [std_preludeScript.sml](std_preludeScript.sml):
 Translations of various useful HOL functions and datatypes, to serve as a
 starting point for further translations.
